\subsection{Lec 09}
    \begin{enumerate}[1]
    \item
        \begin{enumerate}[(1)]
        \item
        $\varliminf\limits_{n\rightarrow{\infty}}\sqrt[n]{\frac{n!}{2^n}}=+\infty$
        \par $\therefore$ $R=+\infty$
        \par $\therefore$ convergence region: $(-\infty,+\infty)$

        \item
        $\varliminf\limits_{n\rightarrow{\infty}}\sqrt[n]{\frac{n}{[3+(-1)^n]^n}}=\frac{1}{4}$
        \par $\therefore$ $R=\frac{1}{4}$
        \par $\because \sum \limits_{n=1}^{\infty} \frac{\left(\frac{1}{2}\right)^{2 n-1}}{2 n-1}$ converge and $|x|=\frac{1}{4}: \sum \limits_{n=1}^{\infty} \frac{1}{2 n} \text { diverge }$
        \par $\therefore$ convergence region: $(-\frac{1}{4},\frac{1}{4})$

        \item
        $\varliminf\limits_{n\rightarrow{\infty}} \sqrt[n]{\frac{n+1}{ \ln (n+1)}}=1$
        \par $\therefore$ $R=1$
        \par $\sum\limits_{n=1}^\infty \frac{ \ln (n+1)}{n+1}$ diverges
        \par $\frac{ \ln (n+1)}{n+1}$ monotonically decreases to $0$ when $n>3$
        \par $\therefore$ $\sum\limits_{n=1}^\infty \frac{(-1)^n  \ln (n+1)}{n+1}$ converges
        \par $\therefore$ divergent when $x=1$, convergent when $x=-1$
        \par $\therefore$ convergence region: $[-1,1)$

        \item
        $|x|=1$: convergent
        \par $|x|>1$: $\lim\limits_{n\rightarrow{\infty}} \frac{|x|^{n^2}}{2^n}=+\infty \neq 0$
        \par $\therefore$ convergence region: $[-1,1]$

        \item
        $\varliminf\limits_{n\rightarrow{\infty}} \sqrt[n]{\frac{n}{3^n+(-2)^n}}=\frac{1}{3}\varliminf\limits_{n\rightarrow{\infty}}\sqrt[n]{\frac{n}{1+(-\frac{2}{3})^n}}=\frac{1}{3}$
        \par $\therefore$ $R=\frac{1}{3}$
        \par $x+1=\frac{1}{3}$: $\sum\limits_{n=1}^\infty \frac{1}{n}$ diverges, $\sum\limits_{n=1}^\infty \frac{(-\frac{2}{3})^n}{n}$ converges $\Rightarrow$ diverges
        \par $x+1=-\frac{1}{3}$: $\sum\limits_{n=1}^\infty \frac{(-1)^n}{n}$ converges, $\sum\limits_{n=1}^\infty \frac{(\frac{2}{3})^n}{n}$ converges $\Rightarrow$ converges
        \par $\therefore$ convergence region: $[-\frac{4}{3},-\frac{2}{3})$

        \item
        $\varliminf\limits_{n\rightarrow{\infty}} \frac{1}{\sqrt[n]{(1+\frac{1}{n})^{n^2}}}=\frac{1}{\me}$
        \par $\therefore$ $R=\frac{1}{\me}$
        \par $\lim\limits_{n\rightarrow{\infty}} \frac{(1+\frac{1}{n})^{n^2}}{\me^n}=\lim\limits_{x\rightarrow{0}} \frac{(1+x)^{\frac{1}{x^2}}}{\me^{\frac{1}{x}}}=\me^{\lim\limits_{x\rightarrow{0}} \ln \frac{(1+x)^{\frac{1}{x^2}}}{\me^{\frac{1}{x}}}}=\me^{\lim\limits_{x\rightarrow{0}}\frac{ \ln (1+x)-x}{x^2}}=\me^{-\frac{1}{2}}\neq 0$
        \par $\therefore$ convergence region: $(-\frac{1}{\me},\frac{1}{\me})$

        \item
        Just let $a\geqslant b$
        \par $\varliminf\limits_{n\rightarrow{\infty}} \sqrt[n]{a^n+b^n}=a\varliminf\limits_{n\rightarrow{\infty}}\sqrt[n]{1+(\frac{b}{a})^n}=a$
        \par $\therefore$ $R=a$
        \par $\lim\limits_{n\rightarrow{\infty}} \frac{a^n}{a^n+b^n}\geqslant \frac{1}{2}$
        \par $\therefore$ convergence region: $(-a,a)$

        \item
        $\varliminf\limits_{n\rightarrow{\infty}} \sqrt[n]{n2^n}=2$
        \par $\therefore$ $R=2$
        \par $|x|=\sqrt{2}$: $\sum\limits_{n=1}^\infty \frac{(-1)^n}{n}$ converges
        \par $\therefore$ convergence region: $[-\sqrt{2},\sqrt{2}]$

        \item
        $1\leqslant \lim\limits_{n\rightarrow{\infty}}\sqrt[2n-1]{\frac{(2n+1)(2n)!!}{(2n-1)!!}}\leqslant \lim\limits_{n\rightarrow{\infty}}\sqrt[2n-1]{\frac{(2n+1)(2n)!!(2n-1)!!}{(2n-1)!!(2n-1)!!}}\leqslant\lim\limits_{n\rightarrow{\infty}}\sqrt[2n-1]{\frac{(2n+1)!}{(2n-1)!}}\\=\lim\limits_{n\rightarrow{\infty}}\sqrt[2n-1]{2n(2n+1)}=1$
        \par $\therefore$ $R=1$
        \par $|x|=1$: $\frac{(2n-1)!!}{(2n+1)(2n)!!}$ monotonically decreases to $0$
        \par $\therefore$ convergent
        \par $\therefore$ convergence region: $[-1,1]$
        \end{enumerate}

    \item
        \begin{enumerate}[(1)]
        \item
        $|x|<\sqrt{A}\Rightarrow x^2<A\Rightarrow$ convergent
        \par $|x|>\sqrt{A}\Rightarrow x^2>A\Rightarrow$ divergent
        \par $\therefore$ $R=\sqrt{A}$

        \item
        $\frac{1}{R}=\varlimsup \limits_{n\to \infty} \sqrt[n]{|a_n+b_n|} \leqslant \varlimsup \limits_{n\to \infty} \sqrt[n]{2\max(|a_n|,|b_n|)} = \max(\frac{1}{A},\frac{1}{B}) $
        \par $\therefore R \geqslant \min(A,B)$

        \item
        $\frac{1}{R}=\varlimsup \limits_{n\to \infty} \sqrt[n]{|a_nb_n|}\leqslant \varlimsup \limits_{n\to \infty} \sqrt[n]{|a_n|}  \varlimsup \limits_{n\to \infty} \sqrt[n]{|b_n|} = \frac{1}{AB}$
        \par $\therefore R \geqslant AB$ 
        \end{enumerate}

    \item
    Let $A_m(x)=\sum\limits_{n=1}^m a_n x^n,\ B_m(x)=\sum\limits_{n=1}^m b_n x^n,\ S_m(x)=\sum\limits_{n=1}^m a_nb_{m-n+1} x^{m+1},\\ R_m(x)=A_m(x)B_m(x)-\sum\limits_{n=1}^m S_n(x),\ M=\sup \limits_{n}[\max (|a_n|,|b_n|)] $
    \par $0<x<1$: $|R_m(x)|<M^2\frac{m^2-m}{2} x^{m+2}$
    \par $\therefore$ $\lim\limits_{m\rightarrow{\infty}} R_m(x)=0,\ 0<x<1$
    \par $\because$ $[0,1]$ is in the uniformly convergence region of $A_m(x),B_m(x),\sum\limits_{n=1}^m S_n(x)$
    \par $\therefore$ $\lim\limits_{m\rightarrow{\infty}} R_m(x)$ is also continuous in $[0,1]$
    \par $\therefore$ $\lim\limits_{m\rightarrow{\infty}} R_m(1)=0$
    \par $\therefore$ $\sum\limits_{n=1}^{\infty} S_n(x)=\lim\limits_{m\rightarrow{\infty}}A_mB_m=AB $\qed
    
    \item
    Apparently $\sum\limits_{n=0}^\infty a_nx^n$ is uniformly convergent in $[0,r)$
    \par $\therefore$ $\int_0^x\lim\limits_{m\rightarrow{\infty}}\sum\limits_{n=0}^m a_nt^n\dif t=\sum\limits_{n=0}^\infty \frac{a_nx^{n+1}}{n+1}$
    \par $\because$ $\sum\limits_{n=0}^\infty \frac{a_nx^{n+1}}{n+1}$ is uniformly convergent in $[0,r]$ and $\frac{a_nx^{n+1}}{n+1}$ is continuous
    \par $\therefore$ $\sum\limits_{n=0}^\infty \frac{a_nx^{n+1}}{n+1}$ is continuous in $[0,r]$
    \par $\therefore$ $\lim\limits_{x\rightarrow{r^-}}\int_0^x\lim\limits_{m\rightarrow{\infty}}\sum\limits_{n=0}^m a_nt^n\dif t$ exists and is equal to $\sum\limits_{n=0}^\infty \frac{a_nx^{n+1}}{n+1} $\qed
    \par $f(x)=-\frac{\ln (1-x)}{x}=\sum\limits_{n=0}^\infty\frac{x^n}{n+1}$
    \par $\because r=\varliminf\limits_{n\rightarrow{\infty}}\sqrt[n]{n+1}=1$ and $\sum\limits_{n=1}^\infty\frac{1}{n^2}$ convergent
    \par $\therefore \sum\limits_{n=1}^\infty\frac{1}{n^2}=-\int_0^1 \frac{\ln (1-x)}{x}\dif x$\qed
    \end{enumerate}

\phantom{1}

\subsection{Lec 10}
    \begin{enumerate}[1]
    \item
    Convergence in $(-\infty,\infty)$ is apparent.
    \par $f^{(2n+1)}(0)=\sum\limits_{m=1}^{\infty} \frac{(-1)^n(2^m)^{2n+1}}{m!}$
    \par $\therefore$ $f(x)\sim\sum\limits_{n=0}^{\infty} \sum\limits_{m=1}^{\infty} \frac{(-1)^n(2^mx)^{2n+1}}{m!(2n+1)!}\sim\sum\limits_{n=0}^{\infty} (\me^{2^{2n+1}}-1)\frac{(-1)^n x^{2n+1}}{(2n+1)!}$
    \par $\because$ $\varliminf\limits_{n\rightarrow{\infty}} \sqrt[2n+1]{\frac{(2n+1)!}{\me^{2^{2n+1}}}}=0$
    \par $\therefore$ $R=0$
    \par $\therefore$ divergent when $x\neq 0$
    
    \item
    $f^{(n)}(0)=\frac{n!}{a^{n+1}}$
    \par $f(x)\sim\sum\limits_{n=0}^{\infty} \frac{x^n}{a^{n+1}}$
    \par $\varliminf\limits_{n\rightarrow{\infty}}\sqrt[n]{|a|^{n+1}}=|a|$
    \par $|\frac{a^n}{a^{n+1}}|=\frac{1}{|a|}\nrightarrow0$
    \par $\therefore$ convergence region: $(-|a|,|a|)$
    
    \item
    $f^{(n)}(2)=\frac{(-1)^{n-1}(n-1)!}{2^n}$
    \par $f(x)\sim  \ln 2+\sum\limits_{n=1}^{\infty} \frac{(-1)^{n-1}(x-2)^n}{2^nn}$
    \par $\varliminf\limits_{n\rightarrow{\infty}}\sqrt[n]{2^nn}=2$
    \par $\sum\limits_{n=1}^\infty \frac{(-1)^n}{n}$ converges and $\sum\limits_{n=1}^\infty \frac{1}{n}$ diverges
    \par $\therefore$ convergence region: $(0,4]$
    
    \item
        \begin{enumerate}[(1)]
        \item
        $f^{(n)}(0)=(\frac{\sin x}{x})^{(n-1)}\big|_{x=0}$
        \par $\because$ $\sin x\sim \sum\limits_{n=0}^\infty \frac{(-1)^nx^{2n+1}}{(2n+1)!}$
        \par $\therefore$ $\frac{\sin x}{x}\sim \sum\limits_{n=0}^\infty \frac{(-1)^nx^{2n}}{(2n+1)!}$
        \par $f^{(2n+1)}(0)=(\frac{\sin x}{x})^{(2n)}\big|_{x=0}=\frac{(-1)^n(2n)!}{(2n+1)!}=\frac{(-1)^n}{2n+1}$
        \par $\therefore$ $f(x)\sim \sum\limits_{n=0}^\infty \frac{(-1)^nx^{2n+1}}{(2n+1)!(2n+1)}$
        \par $R=\varliminf\limits_{n\rightarrow{\infty}} \sqrt[2n+1]{(2n+1)!(2n+1)}=+\infty$
        \par $\therefore$ convergence region: $(-\infty,+\infty)$
        
        \item
        $\cos t^2\sim \sum\limits_{n=0}^\infty \frac{(-1)^nt^{4n}}{(2n)!}$
        \par $\therefore$ $f^{(4n+1)}(0)=(\cos t^2)^{(4n)}\big|_{t=0}=\frac{(-1)^n(4n)!}{(2n)!}$
        \par $\therefore$ $f(x)\sim \sum\limits_{n=0}^\infty \frac{(-1)^nx^{4n+1}}{(2n)!(4n+1)}$
        \par $R=\varliminf\limits_{n\rightarrow{\infty}} \sqrt[4n+1]{(2n)!(4n+1)}=+\infty$
        \par $\therefore$ convergence region: $(-\infty,+\infty)$
        
        \item
        Let $x=\tan t$
        \par $\arctan \frac{2x}{1-x^2}=-\arctan (\tan 2t)=-2\arctan x\sim -2\sum\limits_{n=0}^\infty \frac{(-1)^nx^{2n+1}}{2n+1}$
        \par $\varliminf\limits_{n\rightarrow{\infty}} \sqrt[2n+1]{2n+1}=1$
        \par $|x|=1$: $\sum\limits_{n=0}^\infty \frac{(-1)^n}{2n+1}$ converges
        \par $\therefore$ convergence region: $[-1,1]$ ( with definition: $\arctan (\pm \infty)=\pm \pi$ )
        
        \item
        $f^{(1)}(0)=\frac{1}{\sqrt{1+x^2}}\sim \sum\limits_{n=0}^\infty\frac{(-1)^n(2n-1)!!}{(2n)!!}x^{2n}$
        \par $\therefore$ $f^{(2n+1)}(0)=(\frac{1}{\sqrt{1+x^2}})^{(2n)}\big|_{x=0} =\frac{(-1)^n(2n-1)!!(2n)!}{(2n)!!}$
        \par $\therefore$ $f(x)\sim \sum\limits_{n=0}^\infty\frac{(-1)^n(2n-1)!!}{(2n)!!(2n+1)}x^{2n+1}$
        \par $\varliminf\limits_{n\rightarrow{\infty}} \sqrt[2n+1]{\frac{(2n)!!(2n+1)}{(2n-1)!!}}=1$  (see Lec 09 Prob 1(9))
        \par $\frac{(2n-1)!!}{(2n)!!(2n+1)}$ monotonically decreases to $0$
        \par $\therefore$ converges when $|x|=1$
        \par $\therefore$ convergence region: $[-1,1]$
        \end{enumerate}
        
    \item
        \begin{enumerate}[(1)]
        \item
        $\me^x=\sum\limits_{n=0}^\infty \frac{x^n}{n!},x\in \mathbb{R}$
        \par $\therefore$ $\sum\limits_{n=1}^\infty \frac{x^n}{n!}=\me^x-1,x\in \mathbb{R}$
        
        \item
        $\int_0^x  \ln (1+x)\dif x=(1+x) \ln (1+x)-x$
        \par $\because$ convergence radius of $ \ln (1+x)$'s Maclaurin series is $1$
        \par $\sum\limits_{n=1}^\infty \frac{(-1)^{n+1}x^{n+1}}{n(n+1)}$ converges at $|x|=1$
        \par According to Lec 09 Prob 4, $\sum\limits_{n=1}^\infty \frac{(-1)^{n+1}x^{n+1}}{n(n+1)}=(1+x ) \ln (1+x)-x$ in $[-1,1]$ \\(define $(1+x) \ln (1+x)-x=1$ at $x=-1$)
        
        \item
        \par $\int_0^x f(x)\dif x\sim\sum\limits_{n=1}^\infty nx^n\sim \frac{x}{(x-1)^2}$
        \par $\because$ Convergence radius is $1$ and $f(x)$ diverges at $|x|=1$
        \par $\therefore$ $f(x)=\left[\frac{x}{(x-1)^2}\right]^{'}=\frac{1+x}{(1-x)^3}$ in $(-1,1)$
        
        \item
        Convergence region is $\mathbb{R}$
        \par $\therefore$ $\int_0^x f(x)\dif x = \sum\limits_{n=1}^\infty \frac{x^{2n+1}}{n!}=x(\me^{x^2}-1)$
        \par $\therefore$ $f(x)=[x(\me^{x^2}-1)]^{'}=(2x^2+1)\me^{x^2}-1$
        
        \item
        Let $A=\sum\limits_{n=1}^\infty \frac{2n-1}{2^n}$
        \par $\therefore$ $A=2A-A=1+\sum\limits_{n=1}^\infty  \frac{2n+1}{2^n}    -\sum\limits_{n=1}^\infty \frac{2n-1}{2^n}=3$
        
        \item
        $\sum\limits_{n=0}^\infty \frac{n^2+1}{2^n n!}=\me^{\frac{1}{2}}+\sum\limits_{n=1}^\infty \frac{n}{2^n(n-1)!}=\me^{\frac{1}{2}}+\frac{1}{2}\sum\limits_{n=1}^\infty\frac{(\frac{1}{2})^{n-1}}{(n-1)!}+\frac{1}{4}\sum\limits_{n=2}^\infty \frac{(\frac{1}{2})^{n-2}}{(n-2)!}=\frac{7}{4}\me^{\frac{1}{2}}$
        \end{enumerate}
    \end{enumerate}
