\subsection{P148}
\begin{enumerate}[10]
    \item
    Let $\eta =\sum\limits_{i=1}^n \frac{(-1)^{i-1}}{n}x_i dx_1\wedge \cdots \wedge d \hat{x_i} \wedge \cdots \wedge dx_n$ and verify that $d\eta = \omega $\qed
    \end{enumerate}
    \begin{enumerate}[11]
    \item
    Let $\omega$ be $k-$form
    \par $\therefore$ $d(\omega \wedge \eta)=d\omega\wedge\eta+(-1)^k \omega\wedge d\eta =0$\qed
    \end{enumerate}
    \begin{enumerate}[12]
    \item
    Let $\omega$ be $k-$form and $\eta=d\varphi$
    \par $d[(-1)^k\omega\wedge\varphi]=(-1)^kd\omega\wedge\varphi+\omega\wedge d\varphi=\omega\wedge\eta $\qed
\end{enumerate}
