\subsection{Lec 16}
\begin{enumerate}[1]
    \item 
    \begin{enumerate}[(1)]
        \item 
        $\frac{\dif }{\dif x}F(x)=\me^{x\sqrt{1-\cos^2{x}}}(-\sin{x})-\me^{x\sqrt{1-\sin^2{x}}}(\cos{x})+\int_{\sin{x}}^{\cos{x}}\sqrt{1-y^2}\me^{x\sqrt{1-y^2}}\dif y$
        \par $\phantom{\frac{\dif }{\dif x}F(x)}=\int_{\sin{x}}^{\cos{x}}\sqrt{1-y^2}\me^{x\sqrt{1-y^2}}\dif y-\me^{x|\sin{x}|}\sin{x}-\me^{x|\cos{x}|}\cos{x}$

        \item  
        $\frac{\dif }{\dif x}F(x)=\int_{x^2}^{x^2}f(x,s)\dif s+\int_{0}^{x}2xf(t,x^2)\dif t=\int_{0}^{x}2xf(t,x^2)\dif t$
        
    \end{enumerate}
    \item 
    $F(x)=\frac{1}{2\pi}\int_{0}^{2\pi}\frac{\me^{x\cos{\theta}}(\me^{ix\sin{\theta}}+\me^{-ix\sin{\theta}})}{2}\dif \theta=\frac{1}{2\pi}\int_{0}^{2\pi}\frac{\me^{x\me^{i\theta}}+\me^{x\me^{-i\theta}}}{2}\dif \theta$
    \par $F'(x)=\frac{1}{2\pi}\int_{0}^{2\pi}\me^{i\theta}\frac{\me^{x\me^{i\theta}}}{2}\dif \theta+\frac{1}{2\pi}\int_{0}^{2\pi}\me^{-i\theta}\frac{\me^{x\me^{-i\theta}}}{2}\dif \theta=0$
    \par $\therefore F(x)= $ constï¼Œ$F(x)=F(0)=1$

    \item 
    $I=-\int_0^1\sin{(\ln{x})}\int_a^bx^y\dif y\dif x=-\int_a^b\int_0^1\sin{(\ln{x})}x^y\dif x\dif y$
    \par $\phantom{I}=\int_a^b\frac{1}{(y+1)^2+1}\dif y=\arctan(b+1)-\arctan(a+1)$

    \item 
    $F(x)\phantom{''}=\frac{1}{h^2}\int_0^h\left[\int_0^hf(x+\xi+\eta)\dif \eta\right]\dif \xi=\frac{1}{h^2}\int_x^{x+h}\left[\int_\xi^{\xi+h}f(\eta)\dif \eta\right]\dif \xi$
    \par $F'(x)\phantom{'}=\frac{1}{h^2}\left[\int_{x+h}^{x+2h}f(\eta)\dif \eta-\int_{x}^{x+h}f(\eta)\dif \eta\right]$
    \par $F''(x)=\frac{1}{h^2}\{f(x+2h)-f(x+h)-[f(x+h)-f(x)]\}$
    \par$\phantom{F''(x)} =\frac{f(x+2h)-2f(x+h)+f(h)}{h^2}$\qed
\end{enumerate}

\subsection{Lec 17}

\begin{enumerate}[1]
    \item 
    \begin{enumerate}[(1)]
        \item 
        $\because \left|\frac{\cos{xy}}{x^2+y^2}\right| \leq \frac{1}{a^2+y^2},\ \int_0^{\infty}\frac{1}{a^2+y^2}\dif y$ converges
        \par $\therefore $ uniformly converges
        
        \item 
        $\because \int_0^{+\infty}\frac{\sin{x}}{x}\dif x = \frac{\pi}{2}$ uniformly converges, $ \me^{-\alpha x} $ is about $x$ monotonically decreasing and $\left|\me^{-\alpha x}\right|\leq 1$
        \par $\therefore $ uniformly converges
        
        \item 
        $\because f(x)=\begin{cases}\frac{1}{\sqrt{2\pi}},\ x>0 \\0,\ x=0 \end{cases}$
        \par $\therefore $ not uniformly converges

        
        \item 
        $\int_0^1\frac{1}{x^y}\sin{\frac{1}{x}}\dif x=\int_1^\infty x^{y-2}\sin{x}\dif x$
        \par apply second mean value theorem for definite integrals, $\forall N \in \mathbb{N}^*,\ \exists y=2-\frac{1}{(2N+1)\pi}$
        \par $\int_{2N\pi}^{(2N+1)\pi}x^{y-2}\sin{x}\dif x\leq 2[(2N+1)\pi]^{y-2} = 2[(2N+1)\pi]^{-\frac{1}{(2N+1)\pi}}>1$
        \par $\therefore $ not uniformly converges
        
        \item 
        $ \forall \epsilon > 0,\ \exists \delta < \frac{1}{4} \epsilon^2 $ s.t. $ \int_{y-\delta}^y \frac{\sin xy}{\sqrt{y-x}} \dif x \leq  \int_{y-\delta}^y \frac{1}{\sqrt{y-x}} \dif x =2\sqrt{\delta } \leq \epsilon $
        \par $\therefore $ uniformly converges

        
        \item 
        $\int_0^1x^{p-1}\ln^2{x}\dif x=\int_{-\infty}^0\me^{px}x^2\dif x$
        \par $\because \forall N >0,\ \exists p=\frac{1}{\sqrt[3]{N+1}}$ s.t. $\int_{-\sqrt[3]{N+1}}^{-\sqrt[3]{N}}\me^{px}x^2\dif x>\frac{\me^{-\sqrt[3]{N+1}p}}{3} = \frac{\me^{-1}}{3}$
        \par $\therefore $ not uniformly converges

    \end{enumerate}
    
    
    \item 
    $\because |F(u)|\leq\int_{-\infty}^{+\infty}|f(x)|\dif x = A$
    \par $\therefore F(u)$ is bounded
    \par $\forall \epsilon>0,\ \exists K(\epsilon)>\frac{1}{\epsilon}$, s.t. $\int_{-\infty}^{-K}|f(x)|\dif x+\int_{K}^{+\infty}|f(x)|\dif x<\frac{\epsilon}{3}$
    \par $\exists \delta = \frac{1}{3K^2A}$ when $|u_1-u_2|<\delta$
    \par $|F(u_2)-F(u_1)|=\left|\int_{-\infty}^{+\infty}f(x)(\cos{u_2x}-\cos{u_1x})\dif x\right|$
    \par $\leq \frac{2}{3}\epsilon+2|\int_{-K}^{+K}f(x)\sin \frac{u_2+u_1}{2}x \sin \frac{u_2-u_1}{2}x\dif x|$
    \par $\leq \frac{2}{3}\epsilon +  \frac{1}{3KA}\int_{-K}^{+K}|f(x)\sin \frac{u_2+u_1}{2}x |\dif x$
    \par $\leq \epsilon$
    \par $\therefore $ uniformly continuous\qed
    
    \item 
    $\because \int_0^{+\infty}f(t)\dif t $ uniformly converges,  $\me^{-xt} $ is about $x$ monotonically decreasing and $\left|\me^{-xt}\right|\leq 1\ (x\geq 0)$
    \par $\therefore \int_0^{+\infty}\me^{-xt} f(t)\dif t$ uniformly converges
    \par $\therefore \lim \limits_{x\to 0} \int_0^{+\infty}\me^{-xt} f(t)\dif t = \int_0^{+\infty} f(t)\dif t $\qed
\end{enumerate}
