\subsection{Lec 12}
\begin{enumerate}[1]

    \item [3]
    $\because f'(x)$ monotonically increases in $[0,2\pi]$
    \par $\therefore a_n
    =\frac{1}{\pi}\int_{0}^{2\pi}f(x)\cos nx\dif x=-\frac{1}{n\pi}\int_{0}^{2\pi}f'(x)\sin nx\dif x $
    \par $\phantom{\therefore a_n}=-\frac{1}{n\pi}\sum \limits_{i=0}^{n-1}\int_{\frac{2i}{n}\pi}^{\frac{2i+2}{n}\pi}f'(x)\sin nx\dif x $
    \par $\phantom{\therefore a_n}=-\frac{1}{n\pi}\sum \limits_{i=0}^{n-1}\left[ \int_{\frac{2i}{n}\pi}^{\frac{2i+1}{n}\pi}f'(x)\sin nx\dif x + \int_{\frac{2i+1}{n}\pi}^{\frac{2i+2}{n}\pi}f'(x)\sin nx\dif x \right] $
    \par $\phantom{\therefore a_n}=-\frac{1}{n\pi}\sum \limits_{i=0}^{n-1}\int_{\frac{2i}{n}\pi}^{\frac{2i+1}{n}\pi}\left[ f'(x)-f'(x+\frac{\pi}{n})\right]\sin nx\dif x \geq 0$\qed
\end{enumerate}

\subsection{Lec 13}

\begin{enumerate}[1]
    \item 
    $\phantom{= }\, \lim \limits_{p \rightarrow \infty}\int_{-\pi}^{\pi}f(t)\frac{\cos\frac{t}{2}-\cos pt}{2\sin\frac{t}{2}}\dif t$\\
    $=\lim \limits_{p\rightarrow\infty}\int_{0}^{\pi}[f(t)-f(-t)]\frac{\cos\frac{t}{2}-\cos pt}{2\sin\frac{t}{2}}\dif t$\\
    $= \frac{1}{2}\int_{0}^{\pi}[f(t)-f(-t)]\cot \frac{t}{2}\dif t -\lim \limits_{p\rightarrow\infty}\int_{0}^{\pi}[f(t)-f(-t)]\frac{\cos pt}{2\sin\frac{t}{2}}\dif t$\\
    $= \frac{1}{2}\int_{0}^{\pi}[f(t)-f(-t)]\cot \frac{t}{2}\dif t -\lim \limits_{p \rightarrow \infty} \int_{\delta}^{\pi}[f(t)-f(-t)]\frac{\cos pt}{2\sin\frac{t}{2}}\dif t -\lim \limits_{p \rightarrow \infty} \int_{0}^{\delta}[f(t)-f(-t)]\frac{\cos pt}{2\sin\frac{t}{2}}\dif t$
    \par $\because \frac{f(t)-f(-t)}{2\sin\frac{t}{2}} \in \mathcal{R}[\delta,\pi]$
    \par $\therefore \lim \limits_{p \rightarrow \infty} \int_{\delta}^{\pi}[f(t)-f(-t)]\frac{\cos pt}{2\sin\frac{t}{2}}\dif t=0$
    \par $\because f(t)$ is continuous and has unilateral derivative at $t=0$
    \par $\therefore \exists \delta > 0,\ M>0$ s.t. when $t \in (0,\delta)$, $-M<\frac{f(t)-f(-t)}{2\sin\frac{t}{2}}\cos pt < M $
    \par $\therefore 0=\lim \limits_{\delta \rightarrow 0} -M\delta \leq  \lim \limits_{\delta \rightarrow 0} \lim \limits_{p \rightarrow \infty}  \int_{0}^{\delta}[f(t)-f(-t)]\frac{\cos pt}{2\sin\frac{t}{2}}\dif t\leq \lim \limits_{\delta \rightarrow 0}M\delta =0$
    \par $\therefore  \lim \limits_{p \rightarrow \infty}\int_{-\pi}^{\pi}f(t)\frac{\cos\frac{t}{2}-\cos pt}{2\sin\frac{t}{2}}\dif t = \frac{1}{2}\int_{0}^{\pi}[f(t)-f(-t)]\cot \frac{t}{2}\dif t$\qed

    \item 
    
    \begin{enumerate}[(1)]
        \item 
        \label{(1)}
        \par $f(x)\backsim\frac{a_0}{2}+\sum \limits_{n=1}^{\infty}a_n\cos nx $
        \par $a_0=\frac{2}{\pi}\int_0^{\pi}f(x)\dif x=\frac{2\pi^2}{3}$
        \par $a_n=\frac{2}{\pi}\int_0^{\pi}f(x)\cos nx\dif x=(-1)^n\frac{4}{n^2}$
        \par $f(x) =  \frac{\pi^2}{3} + 4\sum \limits_{n=1}^{\infty} \frac{(-1)^n}{n^2} \cos nx$

        \item 
        \par $f(x)\backsim \sum \limits_{n=1}^{\infty}b_n\sin nx$
        \par $b_n=\frac{2}{\pi}\int_0^{\pi}f(x)\sin nx\dif x= - \frac{4}{\pi n^3} + \frac{2(-1)^n}{\pi}\left(\frac{2}{n^3} - \frac{\pi^2}{n}\right)$
        \par $f(x) = \sum \limits_{n=1}^{\infty}\left[\frac{4(-1)^n}{\pi n^3}- \frac{4}{\pi n^3} - \frac{2\pi(-1)^n}{n}  \right]\sin nx$

        \item 
        \par $ f(x)\backsim\frac{a_0}{2}+\sum \limits_{n=1}^{\infty}[a_n\cos nx+b_n\sin nx]$
        \par $a_0=\frac{2}{\pi}\int_0^{\pi}f(x)\dif x=\frac{8\pi^2}{3}$
        \par $a_n=\frac{2}{\pi}\int_0^{\pi}f(x)\cos nx\dif x=\frac{4}{n^2}$
        \par $b_n=\frac{1}{\pi}\int_0^{\pi}f(x)\sin nx\dif x= -\frac{4\pi}{n}$
        \par $f(x) = \frac{4\pi^2}{3} + \sum \limits_{n=1}^{\infty} \left(\frac{4}{n^2} \cos nx -\frac{4\pi}{n} \sin nx\right)$


        \item 
        from (\hyperref[(1)]{1}) $f(x) =  \frac{\pi^2}{3} + 4\sum \limits_{n=1}^{\infty} \frac{(-1)^n}{n^2} \cos nx$
        \par $f(\pi) =  \frac{\pi^2}{3} + 4\sum \limits_{n=1}^{\infty} \frac{1}{n^2} = \pi^2$
        \par $\sum \limits_{n=1}^{\infty} \frac{1}{n^2} = \frac{\pi^2}{6}$
    \end{enumerate}
    

    \item 
    \par $a_0=\frac{\me^{\pi}-\me^{-\pi}}{\pi}$
    \par $a_n=\frac{(-1)^n(\me^{\pi}-\me^{-\pi})}{\pi(n^2+1)}$
    \par $b_n=-\frac{(-1)^nn(\me^{\pi}-\me^{-\pi})}{\pi(n^2+1)}$
    \par $f(x) = \frac{\me^{\pi}-\me^{-\pi}}{\pi}\left[\frac{1}{2}+\sum \limits_{n=1}^{\infty} \frac{(-1)^n}{(n^2+1)} (\cos nx - n \sin nx)\right]$
    \par if $x=\pi,\ \frac{\me^\pi - \me^{-\pi}}{\pi}\left(\frac{1}{2}+\sum \limits_{n=1}^{\infty} \frac{1}{1+n^2} \right)=\frac{1}{2}(\me^\pi - \me^{-\pi})$
    \par $\sum \limits_{n=1}^{\infty}\frac{1}{1+n^2}=\frac{\pi(\me^{\pi}+\me^{-\pi})}{2(\me^{\pi}-\me^{-\pi})}-\frac{1}{2}$

    \item 
    $\because f(x) \in \mathcal{R} $, apply bessel's inequality
    \par $\therefore \sum \limits_{n=1}^{\infty}a_n^2$ and $\sum \limits_{n=1}^{\infty}b_n^2$ convergent
    \par $\because \frac{|a_n|}{n}\leq\frac{1}{2}(a_n^2+\frac{1}{n^2})$ and $\frac{|b_n|}{n}\leq\frac{1}{2}(b_n^2+\frac{1}{n^2})$
    \par $\therefore \sum \limits_{n=1}^{\infty}\frac{a_n}{n}$ and $\sum \limits_{n=1}^{\infty}\frac{b_n}{n}$ convergent\qed
\end{enumerate}
