\subsection{Lec 04}
 \begin{enumerate}[1]
   \item[5]
   Let $b_k$ equal to the sum of $k^{th}$ set of successive $a_n$ which have the same sign
   \par If $n_0$ is in the $k_0^{th}$ set, denote $k(n_0)=k_0$
   \par $\because$ $ \sum\limits_{k=1}^{\infty}b_k \ \text{convergent},\ \lim\limits_{k\rightarrow\infty}b_k=0$ 
   \par $\therefore$ $\forall \varepsilon >0,\  \exists K>0,\  \forall k_1,\ k_2>K,\  |\sum\limits_{k=k_1}^{k_2}b_k|<\varepsilon,\  |b_{k_1}|+|b_{k_2}|<\varepsilon$
   \par $\because $ $\exists N,\  k(N)>K,\ \forall n_1,\ n_2>N,\ |\sum\limits_{n=n_1}^{n_2}a_n|\leqslant\varepsilon+|b_{k(n_1)}|+|b_{k(n_2)}|<2\varepsilon$
   \par $\therefore$ convergent
   \par For $a_n=\frac{(-1)^{[\sqrt{n}]}}{n}$, let $b_k=(-1)^k\sum\limits_{n=(k-1)^2+1}^{k^2}\frac{1}{n}$
   \par $\therefore$ $|b_k|<\frac{2k}{(k-1)^2}$
   \par $\therefore$ $|b_k|$ monotonically decreases to $0$ and $\sgn (\frac{b_k}{b_{k-1}})=-1$
   \par $\therefore$ $b_k$ converges
   But $|a_n|=\frac{1}{n}$
   \par $\therefore$ conditionally convergent

   \item[8]
   $\forall \varepsilon >0, \exists N>0, \forall n_1,n_2>N$, $\max \{|\sum\limits_{n=n_1}^{n_2}n(a_n-a_{n-1})|, |n_1a_{n_1-1}| ,\ |n_2a_{n_2}|\}<\varepsilon$
   \par $\therefore$ $|\sum\limits_{n=n_1}^{n_2-1}a_n|=|\sum\limits_{n=n_1}^{n_2}n(a_n-a_{n-1})+n_1a_{n_1-1}-n_2a_{n_2}|<3\varepsilon$
   \par $ \therefore \ $ convergent \qed
   \end{enumerate}

\subsection{Lec 05}
    \begin{enumerate}[1]
        \item[3]
        \begin{enumerate}[(1)]
            \item $x_{n+1}-x_n=\frac{\ln (n+1)}{n+1} - \frac{1}{2}\left[\ln ^2(n+1)-\ln ^2n\right]=\frac{\ln (n+1)}{n+1} - \int_n^{n+1} \frac{\ln x}{x} \dif x$
            \par  $\frac{\ln x}{x}$ is monotonically decreasing over $[\me ,\ +\infty) $
            \par if $n>3,\  \frac{\ln (n+1)}{n+1}<\int_n^{n+1} \frac{\ln x}{x} \dif x < \frac{\ln n}{n} $
            \par $\therefore x_{n+1}<x_n,\  x_n $ monotonically decreasing
            \par $ x_n =  \sum\limits_{k=1}^n \frac{\ln k}{k} -\frac{1}{2}\left(\ln n \right)^2 = \sum\limits_{k=1}^n \frac{\ln k}{k} - \int_1^{n} \frac{\ln x}{x} \dif x $
            \par $\phantom{x_n} = \sum\limits_{k=1}^2 \frac{\ln k}{k} - \int_1^{3} \frac{\ln x}{x} \dif x + \sum\limits_{k=3}^n \frac{\ln k}{k} - \int_3^{n} \frac{\ln x}{x} \dif x>  \frac{\ln 2}{2} - \ln ^2 3 $
            \par $\therefore $ convergence

            \item $x_{n+1}-x_n = \frac{1}{\sqrt{n+1}} -2\sqrt{n+1} -2\sqrt{n} < 0$
            \par $\therefore x_n $ monotonically decreasing
            \par $ \sqrt{n} = \sqrt{n} -\sqrt{n-1} + \sqrt{n-1} -\sqrt{n-2} + \cdots + \sqrt{2} -\sqrt{1} + 1 $
            \par $ \phantom{\sqrt{n}}= \frac{1}{\sqrt{n} + \sqrt{n-1}} + \frac{1}{\sqrt{n-1} + \sqrt{n-2}}  + \cdots + \frac{1}{\sqrt{2} + \sqrt{1}}  + 1 $
            \par $ \phantom{\sqrt{n}} < \frac{1}{2}\left( \frac{1}{ \sqrt{n-1}} + \frac{1}{ \sqrt{n-2}}  + \cdots + \frac{1}{ \sqrt{1}}\right) + 1 $
            \par $ x_n> 1 +\frac{1}{\sqrt{2}}+\cdots +\frac{1}{\sqrt{n}}-\left( \frac{1}{ \sqrt{n-1}} + \frac{1}{ \sqrt{n-2}}  + \cdots + \frac{1}{ \sqrt{1}}+2\right) =-2 + \frac{1}{\sqrt{n}} > -2 $
            \par $\therefore $ convergence
        \end{enumerate}

        \item[4]
        $\sum\limits_{n=0}^\infty |x|^n =\frac{1}{1-|x|},\ \sum\limits_{n=0}^\infty |y|^n =\frac{1}{1-|y|}\text{ (both absolutely convergent)}$
        \par $\therefore$ $\sum\limits_{n=1}^\infty (x^{n-1}+x^{n-2}y+ \cdots +y^{n-1})=\sum\limits_{n=0}^\infty x^n\sum\limits_{n=0}^\infty y^n=\frac{1}{(1-x)(1-y)}$\qed

        \item[5]
        $\lim\limits_{n\rightarrow{\infty}}\sqrt[n]{n!}=\infty$
        \par $\therefore$ radius of convergence is $\infty$
        \par $\therefore$ $\sum\limits_{n=0}^\infty \frac{x^n}{n!}=\me^x,\ \sum\limits_{n=0}^\infty \frac{y^n}{n!}=\me^y \text{ both absolutely convergent}$
        \par $\therefore$ $\sum\limits_{n=0}^\infty \frac{x^n}{n!}\sum\limits_{n=0}^\infty \frac{y^n}{n!}=\me ^{x+y}=\sum\limits_{n=0}^\infty \frac{(x+y)^n}{n!}$\qed
    \end{enumerate}

\subsection{Lec 06}
    \begin{enumerate}[1]
        \item
            \begin{enumerate}[(1)]
                \item
                Let $p_n=q_n=1,\ \prod\limits_{n=1}^\infty (p_n+q_n)=\prod\limits_{n=1}^\infty 2 =\infty$
                \par $\therefore$ divergent

                \item
                $\prod\limits_{n=1}^\infty p_n,\ \prod\limits_{n=1}^\infty q_n$ converge
                \par $\Rightarrow \sum\limits_{n=1}^\infty \ln p_n,\ \sum\limits_{n=1}^\infty \ln q_n$ converge
                \par $\Rightarrow \sum\limits_{n=1}^\infty (\ln p_n+\ln q_n)$ converges
                \par $\Rightarrow \sum\limits_{n=1}^\infty \ln (p_nq_n)$ converges
                \par $\Rightarrow \prod\limits_{n=1}^\infty p_nq_n$ converges

                \item
                Let $q_n=p_n$ and use conclusion of previous problem
                \par $\therefore$ convergent

                \item
                $\prod\limits_{n=1}^\infty q_n$ converges
                \par $\Rightarrow \sum\limits_{n=1}^\infty \ln q_n$ converges
                \par $\Rightarrow -\sum\limits_{n=1}^\infty \ln q_n$ converges
                \par $\Rightarrow \prod\limits_{n=1}^\infty \frac{1}{q_n}$ converges
                \par Use conclusion of Lec 06 Prob 1(2), $\prod\limits_{n=1}^\infty \frac{p_n}{q_n}$ converges
            \end{enumerate}

        \item
        Denote $T_n=\prod\limits_{k=1}^{n} (1+u_k),\ S_n=\sum\limits_{k=1}^{n} u_k,\  S'_n=\sum\limits_{k=1}^{n} (u_k)^2$
        \par $\therefore$ $S_{2n}=\sum\limits_{k=1}^n\frac{1}{k}\rightarrow \infty,\ S'_{2n}>2\sum\limits_{k=1}^n\frac{1}{k}\rightarrow \infty$
        \par $\because$ $\lim\limits_{n\rightarrow{\infty}}u_{2n-1}=\lim\limits_{n\rightarrow{\infty}}u_{2n}=0$
        \par $\therefore$ $S_n,\ S'_n$ diverges
        \par $\because$ $(1+u_{2k-1})(1+u_{2k})=1-\frac{1}{k^{\frac{3}{2}}}$
        \par $\therefore$ $T_{2n}$ converges, let A denote its limit
        \par $\therefore$ $\forall \varepsilon >0,\exists N_1>0,\forall n>N_1,\  |T_{2n}-A|<\varepsilon$
        \par And $\lim\limits_{n\rightarrow{\infty}}\frac{T_{2n+1}}{T_{2n}}=u_{2n+1}+1=1$
        \par $\therefore$ for $\varepsilon >0,\ \exists N_2>0,\ \forall n>N_2,\ |T_{2n+1}-T_{2n}|<\varepsilon$
        \par $\therefore$ $\forall \varepsilon >0,\ \exists N=\max \{2N_1+10,\ 2N_2+10\}>0,\ \forall n>N,\  |T_{n}-A|<2\varepsilon$
        \par $\therefore$ $T_{n}$ converges\qed

        \item
            \begin{enumerate}[(1)]
                \item
                $\lim\limits_{n\rightarrow{\infty}}\frac{\ln [(\frac{n^2-1}{n^2+1})^p]}{\frac{1}{n^2}}=\lim\limits_{n\rightarrow{\infty}}\frac{p\ln (1-\frac{2}{n^2+1})}{\frac{1}{n^2}}=-2p$
                \par $\therefore$ convergent

                \item
                $\lim\limits_{n\rightarrow{\infty}}\frac{\ln \sqrt[n]{1+\frac{1}{n}}}{\frac{1}{n^2}}=\lim\limits_{n\rightarrow{\infty}}\frac{\frac{1}{n}\ln (1+\frac{1}{n})}{\frac{1}{n^2}}=1$
                \par $\therefore$ convergent

                \item
                $\lim\limits_{n\rightarrow{\infty}}\frac{\ln \sqrt[n]{\ln (n+x)-\ln n}}{\frac{1}{n}}=\lim\limits_{n\rightarrow{\infty}}\frac{\frac{1}{n}\ln \ln (1+\frac{x}{n})}{\frac{1}{n}}=-\infty$
                \par $\therefore$ divergent

                \item
                $\lim\limits_{n\rightarrow{\infty}}\frac{\ln \frac{n^2-4}{n^2-1}}{\frac{1}{n^2}}=\lim\limits_{n\rightarrow{\infty}}\frac{\ln \left(1-\frac{3}{n^2-1}\right)}{\frac{1}{n^2}}=-3$
                \par $\therefore$ convergent

                \item
                $\ln a^{\frac{(-1)^n}{n}}=\frac{(-1)^n}{n}\ln a$
                \par $\because$ $\frac{1}{n}$ monotonically decreases to 0
                \par $\therefore$ $\sum\limits_{n=1}^\infty \frac{(-1)^n}{n}\ln a$ converges
                \par $\therefore$ convergent

                \item
                $\because$ $\prod\limits_{k=1}^n \sqrt{\frac{k+1}{k+2}}=\sqrt{\frac{2}{n+2}}\rightarrow 0$
                \par $\therefore$ divergent
            \end{enumerate}

        \item[5]
        Due to convergence $\lim\limits_{n\rightarrow{\infty}}a_n=0$
        \par $\tan (\frac{\pi}{4}+x)=1+Ax+o(x),\  A=\tan '(\frac{\pi}{4})>0$
        \par $\therefore$ $\lim\limits_{n\rightarrow{\infty}}\frac{|\ln [\tan (\frac{\pi}{4}+a_n)]|}{|a_n|}=A$
        \par $\therefore$ $\sum\limits_{n=1}^\infty \ln [\tan (\frac{\pi}{4}+a_n)]$ converges
        \par $\therefore$ convergent\qed
    \end{enumerate}
