
\subsection{Lec 01}
\begin{enumerate}[1]
	\item[1]
	Use reduction to absurdity. Suppose \(\lim \limits_{n \rightarrow \infty} a_{n} \neq 0\) or doesn't exist.
	\par \(\therefore \exists \varepsilon>0,\)
	\(\forall N_{1}>0,\  \exists n>N_{1},\ \left|a_{n}\right|>3 \varepsilon .\) For such \(\varepsilon,\ \exists N_{2}>0,\ \forall n>N_{2},\ \left|a_{2 n}+2 a_{n}\right|<\varepsilon\)
	\par \(\therefore \exists N>N_{2},\ \left|a_{N}\right|>3 \varepsilon\) and \(\left|a_{2 N}+2 a_{N}\right|<\varepsilon \) 
	\par \(\therefore \left|a_{2 N}\right|>5 \varepsilon .\) similarly,
	\(\left|a_{4 N}\right|>9 \varepsilon\) and then \(\left|a_{2^{p} N}\right|>\left(2^{p+1}+1\right) \varepsilon\) for \(p \in \mathbb{N},\) which contradict the boundedness of \(a_{n} \)
	$\qedhere$ \qed
	
	\item[2]
	Let \(a_{n}=\frac{2}{3}+b_{n} .\) So \(\lim \limits_{n \rightarrow \infty}\left(b_{2 n}+2 b_{n}\right)=0 .\) According to the conclusion of
	previous problem, \(\lim \limits_{n \rightarrow \infty} b_{n}=0,\) and \(\lim \limits_{n \rightarrow \infty} a_{n}=\frac{2}{3}\) is evident.\qed

	\item[3]
\begin{enumerate}[(1)]
	\item 
	\(\because x_{n+2}=1+\frac{1}{x_{n+1}}=1+\frac{1}{1+\frac{1}{x_{n}}}=1+\frac{x_{n}}{1+x_{n}}\) and using mathematical induction: \(x_{n}>0\)\\
	\(\therefore\) for \(n \geqslant 3,\ 1<x_{n}<2\)\\
	\(\therefore 1 \leqslant \varliminf \limits_{n \rightarrow \infty} x_{n} \leqslant \varlimsup \limits_{n \rightarrow \infty} x_{n}  \leqslant 2\) \qed

	\item 
	\(\because\) for \(n \geqslant 3,\ \left|\frac{x_{n+2}-x_{n+1}}{x_{n+1}-x_{n}}\right|=\left|-\frac{1}{x_{n}+1}\right|<\frac{1}{2}\)\\
	\(\therefore x_{n}\) is a Cauchy sequence	\\
	Calculate the positive fixed point of equation \(x^{*}=1+\frac{1}{x^{*}}\)\\
	\(\therefore \lim \limits_{n \rightarrow \infty} x_{n}=x^{*}=\frac{1+\sqrt{5}}{2}\)


\end{enumerate}

	\item[5]

\begin{enumerate}[(1)]
	\item 
	\(\because \lim \limits_{n \rightarrow \infty} x_{n}+\varlimsup \limits_{n \rightarrow \infty} y_{n} \)\\
	\(= \varliminf \limits_{n \rightarrow \infty} x_{n}+\varlimsup \limits_{n \rightarrow \infty} y_{n} \leqslant \varlimsup \limits_{n \rightarrow \infty}\left(x_{n}+y_{n}\right) \leqslant \varlimsup \limits_{n \rightarrow \infty} x_{n}+\varlimsup \limits_{n \rightarrow \infty} y_{n}\)\\
	\(=\lim \limits_{n \rightarrow \infty} x_{n}+ \varlimsup \limits_{n \rightarrow \infty} y_{n}\)\qed

	\item 
	The proof for \(\varlimsup \limits_{n \rightarrow \infty} y_{n}=\pm \infty\) is direct. Suppose \(\varlimsup \limits_{n \rightarrow \infty} y_{n}=A .\)\\
	\(\forall \varepsilon_{1}>0, \exists N_{1}\left(\varepsilon_{1}\right)>0,\  \forall n>N_{1}\left(\varepsilon_{1}\right),\  y_{n}<A+\varepsilon_{1},\) and \(\exists\left\{y_{n_{k}^{\varepsilon_{1}}}\right\},\  y_{n_{k}^{\varepsilon_{1}}}>\)	\(A-\varepsilon_{1}\)\\
	\(\forall \varepsilon_{2}>0,\ \exists N_{2}\left(\varepsilon_{2}\right)>0,\  \forall n>N_{2}\left(\varepsilon_{2}\right),\ \left|x_{n}-x^{*}\right|<\varepsilon_{2},\  x^{*}=\lim \limits_{n \rightarrow \infty} x_{n}\)\\
	\(\forall \varepsilon>0,\ \exists \varepsilon_{1}>0,\  \varepsilon_{2}>0,\ \forall \delta_{1} \in\left(0, \varepsilon_{1}\right),\  \delta_{2} \in\left(-\varepsilon_{2}, \ \varepsilon_{2}\right),\) s.t. \(0 \leqslant \frac{\delta_{1}}{x^{*}+\delta_{2}}-\)
	\(\frac{A \delta_{2}}{x^{*}\left(x^{*}+\delta_{2}\right)}<\varepsilon,\) and \(0 \leqslant \frac{\delta_{1}}{x^{*}}+\frac{\left(A-\delta_{1}\right) \delta_{2}}{x^{*}\left(x^{*}+\delta_{2}\right)}<\varepsilon\)\\
	\(\therefore\) for \(\forall \varepsilon>0,\  \exists N=\max \left(N_{1}\left(\varepsilon_{1}\right),\  N_{2}\left(\varepsilon_{2}\right)\right),\  \forall n>N,\ \left(x_{n} y_{n}\right)>x^{*} A+\varepsilon\) \\
	and \(\exists\left\{y_{n_{k}^{\varepsilon_{1}}} x_{n_{k}^{\varepsilon_{1}}}\right\},\  y_{n_{k}^{\varepsilon_{1}}} x_{n_{k}^{\varepsilon_{1}}}>x^{*} A-\varepsilon\)\qed
\end{enumerate}

	\item[6]

\begin{enumerate}[(1)]
	\item 
	\(\sup \limits_{k \geqslant n} a_{k}=1,\  \inf \limits_{k \geqslant 2 n} a_{k}=\inf \limits_{k \geqslant 2 n+1} a_{k}=a_{2 n+1}=\frac{1}{2^{-2 n-1}-1}\)\\
	\(\therefore \varlimsup \limits_{n \rightarrow \infty}  a_{n}=\lim \limits_{n \rightarrow \infty} \sup \limits_{k \geqslant n} a_{k}=1, \ \varliminf \limits_{n \rightarrow \infty} a_{n}=\lim \limits_{n \rightarrow \infty} \inf \limits_{k \geqslant n} a_{k}=-1\)

	\item 
	\(\sup \limits_{k \geqslant 2 n} a_{k}=\sup \limits_{k \geqslant 2 n-1} a_{k}=a_{2 n}=1+\frac{1}{2 n}\)\\
	\(\inf \limits_{k \geqslant 2 n} a_{k}=\inf \limits_{k \geqslant 2 n+1} a_{k}=a_{2 n+1}=-1-\frac{1}{2 n+1}\)

	\(\therefore \varlimsup \limits_{n \rightarrow \infty}  a_{n} = \lim \limits_{n \rightarrow \infty} \sup \limits_{k \geqslant n} a_{k}=1,\  \varliminf \limits_{n \rightarrow \infty} a_{n}=\lim \limits_{n \rightarrow \infty} \inf \limits_{k \geqslant n} a_{k}=-1\)

	\item 
	\(\left|a_{n}\right|=\frac{1}{n} \rightarrow 0\)\\
	\(\therefore \varlimsup \limits_{n \rightarrow \infty} a_{n}=\varliminf \limits_{n \rightarrow \infty} a_{n}=\lim \limits_{n \rightarrow \infty} a_{n}=0\)

	\item 
	For a period of \(n=0 \sim 9 \bmod 10,\) maximum \(a_{n}\) is \(\sin \frac{2 \pi}{5},\) minimum \(a_{n}\) is
	\(-\sin \frac{2 \pi}{5}\)\\
	\(\therefore \varlimsup \limits_{n \rightarrow \infty} a_{n}=\lim \limits_{n \rightarrow \infty} \sup \limits_{k \geqslant n} a_{k}=\sin \frac{2 \pi}{5},\ \varliminf \limits_{n \rightarrow \infty} a_{n}=\lim \limits_{n \rightarrow \infty} \inf \limits_{k \geqslant n} a_{k}=-\sin \frac{2 \pi}{5}\)

\end{enumerate}

\end{enumerate}

\subsection{Lec 02}

\begin{enumerate}[1]
	\item[1]
	Suppose \(\varlimsup \limits_{n \rightarrow \infty} na_{n}>0 .\) Then just suppose \( \varlimsup \limits_{n \rightarrow \infty} na_{n} \geqslant 1\)\\
	\(\therefore \exists\left\{a_{n_{k}}\right\},\ a_{n_{k}} \geqslant \frac{1}{n_{k}}\)\\
	Then \(\exists\left\{a_{n_{k_{l}}}\right\},\ n_{k_{l+1}} \geqslant 2 n_{k_{l}}\)\\
	\(\therefore \sum\limits_{n=1}^{\infty} a_{n} \geqslant \sum\limits_{l=2}^{\infty}\left(\frac{n_{k_{l}}}{2} \frac{1}{n_{k_{l}}}\right)=\infty\)\\
	\(\therefore \varlimsup \limits_{n \rightarrow \infty} n a_{n}=0\)\\
	\(\because \varliminf \limits_{n \rightarrow \infty}  n a_{n} \geqslant 0\)\\
	\(\therefore \lim \limits_{n \rightarrow \infty}  n a_{n}=0\)
	

	\item[3]

\begin{enumerate}[(1)]
	\item 	
	\(\because 0 \leqslant \frac{1}{(5 n-4)(5 n+1)} \leqslant \frac{1}{n^{2}}\)\\
	\(\therefore\) absolutely convergent

	\item 	
	\(\because \lim \limits_{n \rightarrow \infty} a_{n}=\frac{1}{2} \neq 0\)\\
	\(\therefore\) divergent

	\item 	
	\(\because 0 \leqslant \frac{1}{2^{n}}+\frac{1}{3^{n}} \leqslant \frac{1}{2^{n-1}}\)\\
	\(\therefore\) absolutely convergent

	\item 	
	\(\because 0 \leqslant \frac{1}{(3 n-2)(3 n+1)} \leqslant \frac{1}{n^{2}}\)\\
	\(\therefore\) absolutely convergent

	\item 	
	\(\because \lim \limits_{n \rightarrow \infty} a_{n}=1 \neq 0\)\\
	\(\therefore\) divergent


\end{enumerate}

	\item[4]	
	
\begin{enumerate}[(1)]
	\item 
	\(\forall \varepsilon>0,\  \exists N>\log _{|q|} \frac{\varepsilon(1-|q|)}{A},\  \forall n_{1},\  n_{2}>N\)\\
 	\(\sum\limits_{n=n_{1}}^{n_{2}}\left|a_{n} q^{n}\right| \leqslant A \sum\limits_{n=n_{1}}^{n_{2}}|q|^{n}=A|q|^{n_{1}} \frac{1-|q|^{n_{2}-n_{1}+1}}{1-|q|}<\varepsilon\)\\
	\(\therefore\) absolutely convergent

	\item 
	\(\because a_n=\frac{1}{3 n-2}+\frac{1}{3 n-1}-\frac{1}{3 n}>\frac{1}{3 n}\)\\
	\(\therefore \exists \varepsilon=1>0,\  \forall N>0,\  \exists n_{1} >N,\ n_2=3n_1+10>N	\)\\
	\(\sum\limits_{n=n_{1}}^{n_{2}} a_{n}>\sum\limits_{n=n_1}^{n_2} \frac{1}{3 n}>\frac{2n_2}{3}\frac{1}{3n_2}>\frac{2}{9}\)\\
	\(\therefore\) divergent


\end{enumerate}
	\item[5]   	
	
	Let \(b_{k}=\sum\limits_{n=n_{k-1}+1}^{n_{k}} a_{n}\)\\
	\(\therefore \forall \varepsilon>0,\ \exists K>0,\ \forall k_{1},k_{2}>K,\ \left|\sum\limits_{k=k_{1}}^{k_{2}} b_{k}\right|<\varepsilon\)\\
	\(\therefore \exists N>n_{K+1}+1,\  \forall n_{1}, n_{2}>N,\ \left|\sum\limits_{n=n_{1}}^{n_{2}} a_{n}\right|<\left|\sum\limits_{k=K}^{\infty} b_{k}\right| \leqslant \varepsilon\)\\
	\(\therefore\) absolutely convergent
	
\end{enumerate}